Rule_TranslationValidation/match_GhostMoveLeft.bpl
@@ -1,4 +1,4 @@
-procedure match_GhostMoveLeft() returns (res: Seq ref)
+procedure match_GhostMoveLeftTest() returns (res: Seq ref)
 ensures res==Seq#Empty() ==> (forall i: int :: inRange(i,0,Seq#Length(findPatterns_GhostMoveLeft($srcHeap)))==>	
 !(   read($srcHeap,Seq#Index(Seq#Index(findPatterns_GhostMoveLeft($srcHeap),i),0),pacman$GameState.STATE) == 4
 	 && read($srcHeap,Seq#Index(Seq#Index(findPatterns_GhostMoveLeft($srcHeap),i),5),pacman$Action.DONEBY) == 2
@@ -70,7 +70,7 @@ var cursor: Seq ref;
 
 
 
-procedure match_filter_GhostMoveLeft(s:ref, rec:ref, ghost:ref, grid2:ref, grid1:ref, act:ref) returns(r: bool);
+procedure match_filter_GhostMoveLeft(s:ref, rec:ref, ghost:ref, grid2:ref, grid1:ref, act:ref) returns(r: bool)
  requires s != null && read($srcHeap,s,alloc) && dtype(s) == pacman$GameState;
  requires rec != null && read($srcHeap,rec,alloc) && dtype(rec) == pacman$Record;
  requires ghost != null && read($srcHeap,ghost,alloc) && dtype(ghost) == pacman$Ghost;
@@ -86,7 +86,118 @@ procedure match_filter_GhostMoveLeft(s:ref, rec:ref, ghost:ref, grid2:ref, grid1
 	 && read($srcHeap,act,pacman$Action.DONEBY) == 2
 	 && read($srcHeap,act,pacman$Action.FRAME) == read($srcHeap, rec, pacman$Record.FRAME)
 	 && read($srcHeap,act,pacman$Action.DIRECTION)==1);
-	 
+{
+
+var s#5: ref;
+var rec#5: ref;
+var ghost#5: ref;
+var grid1#5: ref;
+var grid2#5: ref;
+var act#5: ref;
+var stk: Seq BoxType;
+
+var b#4: bool;
+var b#11: bool;
+var b#19: bool;
+
+var b#4#Box: BoxType;
+var b#11#Box: BoxType;
+var b#19#Box: BoxType;
+
+s#5,rec#5,ghost#5,grid2#5,grid1#5,act#5 := s, rec, ghost, grid2, grid1, act;
+
+stk := OpCode#Aux#InitStk();
+
+Label_0:
+	 // 0: LOAD 0, 0 (s: P!GameState)
+	call stk := OpCode#Load(stk, s#5);
+	 // 1: GET (fieldname: STATE)
+	assert Seq#Length(stk) >= 1;
+	assert $Unbox(Seq#Index(stk, Seq#Length(stk)-1)) != null;
+	stk := Seq#Build(Seq#Take(stk, Seq#Length(stk)-1), $Box($srcHeap[$Unbox(Seq#Index(stk, Seq#Length(stk)-1)), FieldOfDecl(dtype($Unbox(Seq#Index(stk, Seq#Length(stk)-1))), _Field$STATE): Field (int)]));
+	 // 2: PUSH (intValue: 4)
+	call stk := OpCode#Pushi(stk, 4);
+	 // 3: INVOKE (argcount: 1) (opname: =~)
+	call stk := Native#OCLOperation#MatchingOperator
+		(stk, 
+		$Unbox(Seq#Index(stk,Seq#Length(stk)-1)): int,
+		$Unbox(Seq#Index(stk,Seq#Length(stk)-2)): int);
+	 // 4: IFN 10
+	b#4 := $Unbox(OpCode#Top(stk));
+	call stk := OpCode#Pop(stk);
+	if(!b#4){goto Label_10;}
+	 // 5: LOAD 0, 5 (act: P!Action)
+	call stk := OpCode#Load(stk, act#5);
+	 // 6: GET (fieldname: DONEBY)
+	assert Seq#Length(stk) >= 1;
+	assert $Unbox(Seq#Index(stk, Seq#Length(stk)-1)) != null;
+	stk := Seq#Build(Seq#Take(stk, Seq#Length(stk)-1), $Box($srcHeap[$Unbox(Seq#Index(stk, Seq#Length(stk)-1)), FieldOfDecl(dtype($Unbox(Seq#Index(stk, Seq#Length(stk)-1))), _Field$DONEBY): Field (int)]));
+	 // 7: PUSH (intValue: 2)
+	call stk := OpCode#Pushi(stk, 2);
+	 // 8: INVOKE (argcount: 1) (opname: =~)
+	call stk := Native#OCLOperation#MatchingOperator
+		(stk, 
+		$Unbox(Seq#Index(stk,Seq#Length(stk)-1)): int,
+		$Unbox(Seq#Index(stk,Seq#Length(stk)-2)): int);
+	 // 9: GOTO 11
+	goto Label_11;
+Label_10:
+	// 10: PUSHF
+	call stk := OpCode#Pushf(stk);
+Label_11:
+	// 11: IFN 18
+	b#11 := $Unbox(OpCode#Top(stk));
+	call stk := OpCode#Pop(stk);
+	if(!b#11){goto Label_18;}
+	// 12: LOAD 0, 5 (act: P!Action)
+	call stk := OpCode#Load(stk, act#5);
+	// 13: GET (fieldname: FRAME)
+	assert Seq#Length(stk) >= 1;
+	assert $Unbox(Seq#Index(stk, Seq#Length(stk)-1)) != null;
+	stk := Seq#Build(Seq#Take(stk, Seq#Length(stk)-1), $Box($srcHeap[$Unbox(Seq#Index(stk, Seq#Length(stk)-1)), FieldOfDecl(dtype($Unbox(Seq#Index(stk, Seq#Length(stk)-1))), _Field$FRAME): Field (int)]));
+	// 14: LOAD 0, 1 (rec: P!Record)
+	call stk := OpCode#Load(stk, rec#5);
+	// 15: GET (fieldname: FRAME)
+	assert Seq#Length(stk) >= 1;
+	assert $Unbox(Seq#Index(stk, Seq#Length(stk)-1)) != null;
+	stk := Seq#Build(Seq#Take(stk, Seq#Length(stk)-1), $Box($srcHeap[$Unbox(Seq#Index(stk, Seq#Length(stk)-1)), FieldOfDecl(dtype($Unbox(Seq#Index(stk, Seq#Length(stk)-1))), _Field$FRAME): Field (int)]));
+	// 16: INVOKE (argcount: 1) (opname: =~)
+	call stk := Native#OCLOperation#MatchingOperator
+		(stk, 
+		$Unbox(Seq#Index(stk,Seq#Length(stk)-1)): int,
+		$Unbox(Seq#Index(stk,Seq#Length(stk)-2)): int);
+	// 17: GOTO 19
+	goto Label_19;
+Label_18:
+	// 18: PUSHF
+	call stk := OpCode#Pushf(stk);
+Label_19:
+	// 19: IFN 25
+	b#19 := $Unbox(OpCode#Top(stk));
+	call stk := OpCode#Pop(stk);
+	if(!b#19){goto Label_25;}
+	// 20: LOAD 0, 5 (act: P!Action)
+	call stk := OpCode#Load(stk, act#5);
+	// 21: GET (fieldname: DIRECTION)
+	assert Seq#Length(stk) >= 1;
+	assert $Unbox(Seq#Index(stk, Seq#Length(stk)-1)) != null;
+	stk := Seq#Build(Seq#Take(stk, Seq#Length(stk)-1), $Box($srcHeap[$Unbox(Seq#Index(stk, Seq#Length(stk)-1)), FieldOfDecl(dtype($Unbox(Seq#Index(stk, Seq#Length(stk)-1))), _Field$DIRECTION): Field (int)]));
+	// 22: PUSH (intValue: 1)
+	call stk := OpCode#Pushi(stk, 1);
+	// 23: INVOKE (argcount: 1) (opname: =~)
+	call stk := Native#OCLOperation#MatchingOperator
+		(stk, 
+		$Unbox(Seq#Index(stk,Seq#Length(stk)-1)): int,
+		$Unbox(Seq#Index(stk,Seq#Length(stk)-2)): int);
+	// 24: GOTO 26
+	goto Label_26;
+Label_25:
+	// 25: PUSHF
+	call stk := OpCode#Pushf(stk);
+Label_26:
+	r:= $Unbox(OpCode#Top(stk));
+	call stk := OpCode#Pop(stk);
+}	 
 	 
 
 	
