Rule_TranslationValidation/match_Kill.bpl
@@ -1,4 +1,4 @@
-procedure match_Kill() returns (res: Seq ref)
+procedure match_KillTest() returns (res: Seq ref)
 ensures res==Seq#Empty() ==> (forall i: int :: inRange(i,0,Seq#Length(findPatterns_Kill($srcHeap)))==>	
 !(  read($srcHeap,Seq#Index(Seq#Index(findPatterns_Kill($srcHeap),i),0),pacman$GameState.STATE) == 5
 ));
@@ -50,7 +50,7 @@ var cursor: Seq ref;
 		}
 }
 
-procedure match_filter_Kill(s:ref, ghost:ref, pac:ref, grid:ref) returns(r: bool);
+procedure match_filter_Kill(s:ref, ghost:ref, pac:ref, grid:ref) returns(r: bool)
  requires s != null && read($srcHeap,s,alloc) && dtype(s) == pacman$GameState;
  requires ghost != null && read($srcHeap,ghost,alloc) && dtype(ghost) == pacman$Ghost;
  requires pac != null && read($srcHeap,pac,alloc) && dtype(pac) == pacman$Pacman;
@@ -59,3 +59,35 @@ procedure match_filter_Kill(s:ref, ghost:ref, pac:ref, grid:ref) returns(r: bool
  requires read($srcHeap,grid,pacman$Grid.hasEnemy) == ghost;
  ensures r <==> ( 
 		read($srcHeap,s,pacman$GameState.STATE) == 5);
+{
+var s#10: ref;
+var ghost#10: ref;
+var pac#10: ref;
+var grid#10: ref;
+
+var stk: Seq BoxType;
+
+s#10,ghost#10,pac#10,grid#10 := s,ghost,pac,grid;
+
+stk := OpCode#Aux#InitStk();
+
+call stk := OpCode#Load(stk, s#10);
+
+// get GameState.State
+assert Seq#Length(stk) >= 1;
+assert $Unbox(Seq#Index(stk, Seq#Length(stk)-1)) != null;
+stk := Seq#Build(Seq#Take(stk, Seq#Length(stk)-1), $Box($srcHeap[$Unbox(Seq#Index(stk, Seq#Length(stk)-1)), FieldOfDecl(dtype($Unbox(Seq#Index(stk, Seq#Length(stk)-1))), _Field$STATE): Field (int)]));
+
+// push 5
+call stk := OpCode#Pushi(stk, 5);
+
+// invoke =~
+call stk := Native#OCLOperation#MatchingOperator
+	(stk, 
+	$Unbox(Seq#Index(stk,Seq#Length(stk)-1)): int,
+	$Unbox(Seq#Index(stk,Seq#Length(stk)-2)): int);
+
+r:= $Unbox(OpCode#Top(stk));
+call stk := OpCode#Pop(stk);
+
+}
