Rule_TranslationValidation/match_PlayerMoveLeft.bpl
@@ -1,10 +1,12 @@
-procedure match_PlayerMoveLeft() returns (res: Seq ref)
+procedure match_PlayerMoveLeftTest() returns (res: Seq ref)
 ensures res==Seq#Empty() ==> (forall i: int :: inRange(i,0,Seq#Length(findPatterns_PlayerMoveLeft($srcHeap)))==>	
 !(   read($srcHeap,Seq#Index(Seq#Index(findPatterns_PlayerMoveLeft($srcHeap),i),0),pacman$GameState.STATE) == 3
 	 && read($srcHeap,Seq#Index(Seq#Index(findPatterns_PlayerMoveLeft($srcHeap),i),5),pacman$Action.DONEBY) == 1
 	 && read($srcHeap,Seq#Index(Seq#Index(findPatterns_PlayerMoveLeft($srcHeap),i),5),pacman$Action.FRAME) == 
 			read($srcHeap, Seq#Index(Seq#Index(findPatterns_PlayerMoveLeft($srcHeap),i),1), pacman$Record.FRAME)
-	 && read($srcHeap,Seq#Index(Seq#Index(findPatterns_PlayerMoveLeft($srcHeap),i),5),pacman$Action.DIRECTION)==1)
+	 && read($srcHeap,Seq#Index(Seq#Index(findPatterns_PlayerMoveLeft($srcHeap),i),5),pacman$Action.DIRECTION)==1
+	 && !(dtype(read($srcHeap,Seq#Index(Seq#Index(findPatterns_PlayerMoveLeft($srcHeap),i),3), pacman$Grid.hasEnemy))<:pacman$Ghost)
+)
 );
 ensures res!=Seq#Empty() ==> 
        Seq#Contains(findPatterns_PlayerMoveLeft($srcHeap), res) 
@@ -13,6 +15,7 @@ ensures res!=Seq#Empty() ==>
 	&& read($srcHeap,Seq#Index(res,5),pacman$Action.FRAME) == 
 			read($srcHeap, Seq#Index(res,1), pacman$Record.FRAME)
 	&& read($srcHeap,Seq#Index(res,5),pacman$Action.DIRECTION)==1
+	&& !(dtype(read($srcHeap,Seq#Index(res,3), pacman$Grid.hasEnemy))<:pacman$Ghost)
 ;
 {
 var $i: int;
@@ -26,6 +29,9 @@ var act#0: ref;
 
 var P#0: Seq (Seq ref);
 var b#0: bool;
+
+
+
 
 var cursor: Seq ref;
 
@@ -41,7 +47,8 @@ var cursor: Seq ref;
 			 && read($srcHeap,Seq#Index(Seq#Index(P#0,i),5),pacman$Action.DONEBY) == 1
 			 && read($srcHeap,Seq#Index(Seq#Index(P#0,i),5),pacman$Action.FRAME) == 
 					read($srcHeap, Seq#Index(Seq#Index(P#0,i),1), pacman$Record.FRAME)
-			 && read($srcHeap,Seq#Index(Seq#Index(P#0,i),5),pacman$Action.DIRECTION)==1)
+			 && read($srcHeap,Seq#Index(Seq#Index(P#0,i),5),pacman$Action.DIRECTION)==1
+			 && dtype(read($srcHeap,Seq#Index(Seq#Index(P#0,i),3), pacman$Grid.hasEnemy))!=pacman$Ghost)
 			);
 		{
 
@@ -63,14 +70,13 @@ var cursor: Seq ref;
 			$i := $i+1;
 		}
 
-
 }
 
 
 
 
 
-procedure match_filter_PlayerMoveLeft(s:ref, rec:ref, pac:ref, grid2:ref, grid1:ref, act:ref) returns(r: bool);
+procedure match_filter_PlayerMoveLeft(s:ref, rec:ref, pac:ref, grid2:ref, grid1:ref, act:ref) returns(r: bool)
  requires s != null && read($srcHeap,s,alloc) && dtype(s) == pacman$GameState;
  requires rec != null && read($srcHeap,rec,alloc) && dtype(rec) == pacman$Record;
  requires pac != null && read($srcHeap,pac,alloc) && dtype(pac) == pacman$Pacman;
@@ -81,10 +87,193 @@ procedure match_filter_PlayerMoveLeft(s:ref, rec:ref, pac:ref, grid2:ref, grid1:
  requires read($srcHeap,s,pacman$GameState.record) == rec;
  requires read($srcHeap,grid1,pacman$Grid.hasPlayer) == pac;
  requires read($srcHeap,grid1,pacman$Grid.left) == grid2;
+ free requires !(dtype(read($srcHeap,grid2,pacman$Grid.hasEnemy)) <: class._System.array); // # SHOULD BE IN METAMODEL.BPL
  ensures r <==> ( 
 		read($srcHeap,s,pacman$GameState.STATE) == 3
 	 && read($srcHeap,act,pacman$Action.DONEBY) == 1
 	 && read($srcHeap,act,pacman$Action.FRAME) == read($srcHeap, rec, pacman$Record.FRAME)
-	 && read($srcHeap,act,pacman$Action.DIRECTION)==1);
-	 
+	 && read($srcHeap,act,pacman$Action.DIRECTION)==1
+	 && !(dtype(read($srcHeap,grid2, pacman$Grid.hasEnemy))<:pacman$Ghost));
+{
+var s#0: ref;
+var rec#0: ref;
+var pac#0: ref;
+var grid1#0: ref;
+var grid2#0: ref;
+var act#0: ref;
+var stk: Seq BoxType;
+
+var b#4: bool;
+var b#11: bool;
+var b#19: bool;
+var b#26: bool;
+var b#32: bool;
+var b#36: bool;
+
+var obj#33: Seq ref;
+var $i: int;
+
+s#0,rec#0,pac#0,grid2#0,grid1#0,act#0 := s, rec, pac, grid2, grid1, act;
+
+stk := OpCode#Aux#InitStk();
+
+Label_0:
+	 // 0: LOAD 0, 0 (s: P!GameState)
+	call stk := OpCode#Load(stk, s#0);
+	 // 1: GET (fieldname: STATE)
+	assert Seq#Length(stk) >= 1;
+	assert $Unbox(Seq#Index(stk, Seq#Length(stk)-1)) != null;
+	stk := Seq#Build(Seq#Take(stk, Seq#Length(stk)-1), $Box($srcHeap[$Unbox(Seq#Index(stk, Seq#Length(stk)-1)), FieldOfDecl(dtype($Unbox(Seq#Index(stk, Seq#Length(stk)-1))), _Field$STATE): Field (int)]));
+	 // 2: PUSH (intValue: 3)
+	call stk := OpCode#Pushi(stk, 3);
+	 // 3: INVOKE (argcount: 1) (opname: =~)
+	call stk := Native#OCLOperation#MatchingOperator
+		(stk, 
+		$Unbox(Seq#Index(stk,Seq#Length(stk)-1)): int,
+		$Unbox(Seq#Index(stk,Seq#Length(stk)-2)): int);
+	 // 4: IFN 10
+	b#4 := $Unbox(OpCode#Top(stk));
+	call stk := OpCode#Pop(stk);
+	if(!b#4){goto Label_10;}
+	 // 5: LOAD 0, 5 (act: P!Action)
+	call stk := OpCode#Load(stk, act#0);
+	 // 6: GET (fieldname: DONEBY)
+	assert Seq#Length(stk) >= 1;
+	assert $Unbox(Seq#Index(stk, Seq#Length(stk)-1)) != null;
+	stk := Seq#Build(Seq#Take(stk, Seq#Length(stk)-1), $Box($srcHeap[$Unbox(Seq#Index(stk, Seq#Length(stk)-1)), FieldOfDecl(dtype($Unbox(Seq#Index(stk, Seq#Length(stk)-1))), _Field$DONEBY): Field (int)]));
+	 // 7: PUSH (intValue: 1)
+	call stk := OpCode#Pushi(stk, 1);
+	 // 8: INVOKE (argcount: 1) (opname: =~)
+	call stk := Native#OCLOperation#MatchingOperator
+		(stk, 
+		$Unbox(Seq#Index(stk,Seq#Length(stk)-1)): int,
+		$Unbox(Seq#Index(stk,Seq#Length(stk)-2)): int);
+	 // 9: GOTO 11
+	goto Label_11;
+Label_10:
+	// 10: PUSHF
+	call stk := OpCode#Pushf(stk);
+Label_11:
+	// 11: IFN 18
+	b#11 := $Unbox(OpCode#Top(stk));
+	call stk := OpCode#Pop(stk);
+	if(!b#11){goto Label_18;}
+	// 12: LOAD 0, 5 (act: P!Action)
+	call stk := OpCode#Load(stk, act#0);
+	// 13: GET (fieldname: FRAME)
+	assert Seq#Length(stk) >= 1;
+	assert $Unbox(Seq#Index(stk, Seq#Length(stk)-1)) != null;
+	stk := Seq#Build(Seq#Take(stk, Seq#Length(stk)-1), $Box($srcHeap[$Unbox(Seq#Index(stk, Seq#Length(stk)-1)), FieldOfDecl(dtype($Unbox(Seq#Index(stk, Seq#Length(stk)-1))), _Field$FRAME): Field (int)]));
+	// 14: LOAD 0, 1 (rec: P!Record)
+	call stk := OpCode#Load(stk, rec#0);
+	// 15: GET (fieldname: FRAME)
+	assert Seq#Length(stk) >= 1;
+	assert $Unbox(Seq#Index(stk, Seq#Length(stk)-1)) != null;
+	stk := Seq#Build(Seq#Take(stk, Seq#Length(stk)-1), $Box($srcHeap[$Unbox(Seq#Index(stk, Seq#Length(stk)-1)), FieldOfDecl(dtype($Unbox(Seq#Index(stk, Seq#Length(stk)-1))), _Field$FRAME): Field (int)]));
+	// 16: INVOKE (argcount: 1) (opname: =~)
+	call stk := Native#OCLOperation#MatchingOperator
+		(stk, 
+		$Unbox(Seq#Index(stk,Seq#Length(stk)-1)): int,
+		$Unbox(Seq#Index(stk,Seq#Length(stk)-2)): int);
+	// 17: GOTO 19
+	goto Label_19;
+Label_18:
+	// 18: PUSHF
+	call stk := OpCode#Pushf(stk);
+Label_19:
+	// 19: IFN 25
+	b#19 := $Unbox(OpCode#Top(stk));
+	call stk := OpCode#Pop(stk);
+	if(!b#19){goto Label_25;}
+	// 20: LOAD 0, 5 (act: P!Action)
+	call stk := OpCode#Load(stk, act#0);
+	// 21: GET (fieldname: DIRECTION)
+	assert Seq#Length(stk) >= 1;
+	assert $Unbox(Seq#Index(stk, Seq#Length(stk)-1)) != null;
+	stk := Seq#Build(Seq#Take(stk, Seq#Length(stk)-1), $Box($srcHeap[$Unbox(Seq#Index(stk, Seq#Length(stk)-1)), FieldOfDecl(dtype($Unbox(Seq#Index(stk, Seq#Length(stk)-1))), _Field$DIRECTION): Field (int)]));
+	// 22: PUSH (intValue: 1)
+	call stk := OpCode#Pushi(stk, 1);
+	// 23: INVOKE (argcount: 1) (opname: =~)
+	call stk := Native#OCLOperation#MatchingOperator
+		(stk, 
+		$Unbox(Seq#Index(stk,Seq#Length(stk)-1)): int,
+		$Unbox(Seq#Index(stk,Seq#Length(stk)-2)): int);
+	// 24: GOTO 26
+	goto Label_26;
+Label_25:
+	// 25: PUSHF
+	call stk := OpCode#Pushf(stk);
+Label_26:
+	// 26: IFN 47
+	b#26 := $Unbox(OpCode#Top(stk));
+	call stk := OpCode#Pop(stk);
+	if(!b#26){goto Label_47;}
+	// 27: LOAD 0, 3 (grid2: P!Grid)
+	call stk := OpCode#Load(stk, grid2#0);
+	// 28: GET (fieldname: hasEnemy)
+	assert Seq#Length(stk) >= 1;
+	assert $Unbox(Seq#Index(stk, Seq#Length(stk)-1)) != null;
+	stk := Seq#Build(Seq#Take(stk, Seq#Length(stk)-1), $Box($srcHeap[$Unbox(Seq#Index(stk, Seq#Length(stk)-1)), FieldOfDecl(dtype($Unbox(Seq#Index(stk, Seq#Length(stk)-1))), _Field$hasEnemy): Field (ref)]));
+	// 29: DUP
+	call stk := OpCode#Dup(stk);
+	// 30: FINDTYPE (modelname: #native, typename: Collection)
+	call stk := OpCode#FindType(stk, _Native, _Collection);
+	// 31: INVOKE (argcount: 1) (opname: oclIsKindOf)
+	call stk := EMFTVM#OCL#isKindOf(stk);
+	// 32: IFN 43
+	b#32 := $Unbox(OpCode#Top(stk));
+	call stk := OpCode#Pop(stk);
+	if(!b#32){goto Label_43;}
+	// 33: ITERATE 38
+	$i:=0;
+	obj#33 := $Unbox(OpCode#Top(stk));
+	call stk := OpCode#Pop(stk);
+	while($i<Seq#Length(obj#33))
+	  invariant $i <= Seq#Length(obj#33);
+	  invariant (forall i: int:: 0<=i &&i <$i ==>
+			!(dtype(Seq#Index(obj#33,i)) <: pacman$Ghost)
+	  );
+	{
+		stk := Seq#Build(stk, $Box(Seq#Index(obj#33, $i)));
+
+		// 34: FINDTYPE (modelname: P, typename: Ghost)
+		call stk := OpCode#FindType(stk, _P, _Ghost);
+		// 35: INVOKE (argcount: 1) (opname: oclIsKindOf)
+		call stk := EMFTVM#OCL#isKindOf(stk);
+		// 36: IF 40
+		b#36 := $Unbox(OpCode#Top(stk));
+		call stk := OpCode#Pop(stk);
+		if(b#36){goto Label_40;}
+		// 37: ENDITERATE 34
+	}
+	
+	// 38: PUSHF
+	call stk := OpCode#Pushf(stk);
+	// 39: GOTO 45
+	goto Label_45;
+Label_40:
+	// 40: POP
+	call stk := OpCode#Pop(stk);
+	// 41: PUSHT
+	call stk := OpCode#Pusht(stk);
+	// 42: GOTO 45
+	goto Label_45;
+Label_43:
+	// 43: FINDTYPE (modelname: P, typename: Ghost)
+	call stk := OpCode#FindType(stk, _P, _Ghost);
+	// 44: INVOKE (argcount: 1) (opname: oclIsKindOf)
+	call stk := EMFTVM#OCL#isKindOf(stk);
+Label_45:
+	// 45: NOT
+	call stk := OpCode#Not(stk);
+	// 46: GOTO 48
+	goto Label_48;
+Label_47:
+	// 47: PUSHF
+	call stk := OpCode#Pushf(stk);
+Label_48:
+	r:= $Unbox(OpCode#Top(stk));
+	call stk := OpCode#Pop(stk);
+	
+}	 
 
